examples/sys_regs.v
@@ -2,21 +2,21 @@ Require Import isla.base.
 Require Import isla.automation.
 
 Definition sys_regs : list (reg_col_entry * valu) := [
-  (RegColDirect "SCTLR_EL2" , Val_Bits [BV{64} 0x0000000004000002] );
-  (RegColDirect "SCR_EL3" , Val_Bits [BV{32} 0] );
-  (RegColDirect "TCR_EL2" , Val_Bits [BV{64} 0] );
-  (RegColDirect "CFG_ID_AA64PFR0_EL1_EL0" , Val_Bits [BV{4} 1] );
-  (RegColDirect "CFG_ID_AA64PFR0_EL1_EL1" , Val_Bits [BV{4} 1] );
-  (RegColDirect "CFG_ID_AA64PFR0_EL1_EL2" , Val_Bits [BV{4} 1] );
-  (RegColDirect "CFG_ID_AA64PFR0_EL1_EL3" , Val_Bits [BV{4} 1] );
-  (RegColDirect "OSLSR_EL1" , Val_Bits [BV{32} 0] );
-  (RegColDirect "OSDLR_EL1" , Val_Bits [BV{32} 0] );
-  (RegColDirect "EDSCR" , Val_Bits [BV{32} 0] );
-  (RegColDirect "MPIDR_EL1" , Val_Bits [BV{64} 0] );
-  (RegColStruct "PSTATE" "SP" , Val_Bits [BV{1} 1] );
-  (RegColStruct "PSTATE" "EL" , Val_Bits [BV{2} 2] );
-  (RegColStruct "PSTATE" "nRW" , Val_Bits [BV{1} 0] );
-  (RegColStruct "PSTATE" "D" , Val_Bits [BV{1} 1])
+  (RegColDirect "SCTLR_EL2" , RegVal_Base (Val_Bits [BV{64} 0x0000000004000002]) );
+  (RegColDirect "SCR_EL3" , RegVal_Base (Val_Bits [BV{32} 0]) );
+  (RegColDirect "TCR_EL2" , RegVal_Base (Val_Bits [BV{64} 0]) );
+  (RegColDirect "CFG_ID_AA64PFR0_EL1_EL0" , RegVal_Base (Val_Bits [BV{4} 1]) );
+  (RegColDirect "CFG_ID_AA64PFR0_EL1_EL1" , RegVal_Base (Val_Bits [BV{4} 1]) );
+  (RegColDirect "CFG_ID_AA64PFR0_EL1_EL2" , RegVal_Base (Val_Bits [BV{4} 1]) );
+  (RegColDirect "CFG_ID_AA64PFR0_EL1_EL3" , RegVal_Base (Val_Bits [BV{4} 1]) );
+  (RegColDirect "OSLSR_EL1" , RegVal_Base (Val_Bits [BV{32} 0]) );
+  (RegColDirect "OSDLR_EL1" , RegVal_Base (Val_Bits [BV{32} 0]) );
+  (RegColDirect "EDSCR" , RegVal_Base (Val_Bits [BV{32} 0]) );
+  (RegColDirect "MPIDR_EL1" , RegVal_Base (Val_Bits [BV{64} 0]) );
+  (RegColStruct "PSTATE" "SP" , RegVal_Base (Val_Bits [BV{1} 1]) );
+  (RegColStruct "PSTATE" "EL" , RegVal_Base (Val_Bits [BV{2} 2]) );
+  (RegColStruct "PSTATE" "nRW" , RegVal_Base (Val_Bits [BV{1} 0]) );
+  (RegColStruct "PSTATE" "D" , RegVal_Base (Val_Bits [BV{1} 1]))
 ].
 
 Definition sys_regs_map : reg_map :=
