theories/isla_lang.v
@@ -12,6 +12,7 @@ Require Export isla.base isla.bitvector.
 
 
 Definition var_name : Set := Z.
+Definition eq_var_name (v w : var_name) : bool := Z.eqb v w.
 
 Definition register_name : Set := string.
 
@@ -25,23 +26,6 @@ Inductive annot : Type :=
 | Mk_annot : annot.
 
 Definition enum : Set := (enum_id*enum_ctor).
-
-Inductive bvmanyarith : Set := 
- | Bvand : bvmanyarith
- | Bvor : bvmanyarith
- | Bvxor : bvmanyarith
- | Bvadd : bvmanyarith
- | Bvmul : bvmanyarith.
-
-Inductive bvcomp : Set := 
- | Bvult : bvcomp
- | Bvslt : bvcomp
- | Bvule : bvcomp
- | Bvsle : bvcomp
- | Bvuge : bvcomp
- | Bvsge : bvcomp
- | Bvugt : bvcomp
- | Bvsgt : bvcomp.
 
 Inductive bvarith : Set := 
  | Bvnand : bvarith
@@ -59,11 +43,39 @@ Inductive bvarith : Set :=
  | Bvlshr : bvarith
  | Bvashr : bvarith.
 
+Inductive bvcomp : Set := 
+ | Bvult : bvcomp
+ | Bvslt : bvcomp
+ | Bvule : bvcomp
+ | Bvsle : bvcomp
+ | Bvuge : bvcomp
+ | Bvsge : bvcomp
+ | Bvugt : bvcomp
+ | Bvsgt : bvcomp.
+
+Inductive bvmanyarith : Set := 
+ | Bvand : bvmanyarith
+ | Bvor : bvmanyarith
+ | Bvxor : bvmanyarith
+ | Bvadd : bvmanyarith
+ | Bvmul : bvmanyarith.
+
+Inductive binop : Set := 
+ | Eq : binop
+ | Bvarith (bvarith5:bvarith)
+ | Bvcomp (bvcomp5:bvcomp).
+
 Inductive manyop : Set := 
  | And : manyop
  | Or : manyop
  | Bvmanyarith (bvmanyarith5:bvmanyarith)
  | Concat : manyop.
+
+Inductive base_val : Set := 
+ | Val_Symbolic (vvar5:var_name)
+ | Val_Bool (bool5:bool)
+ | Val_Bits (bv5:bvn)
+ | Val_Enum (enum5:enum).
 
 Inductive unop : Set := 
  | Not : unop
@@ -75,37 +87,29 @@ Inductive unop : Set :=
  | ZeroExtend (nat5:N)
  | SignExtend (nat5:N).
 
-Inductive binop : Set := 
- | Eq : binop
- | Bvarith (bvarith5:bvarith)
- | Bvcomp (bvcomp5:bvcomp).
-
-Inductive valu : Set := 
- | Val_Symbolic (vvar5:var_name)
- | Val_Bool (bool5:bool)
- | Val_I (bvi5:Z) (int5:Z)
- | Val_Bits (bv5:bvn)
- | Val_Enum (enum5:enum)
- | Val_String (str5:string)
- | Val_Unit : valu
- | Val_NamedUnit (name5:register_name)
- | Val_Vector (_:list valu)
- | Val_List (_:list valu)
- | Val_Struct (_:list (register_name * valu))
- | Val_Poison : valu.
-
-Inductive exp : Set := 
- | Val (valu5:valu) (annot5:annot)
- | Unop (unop5:unop) (exp5:exp) (annot5:annot)
- | Binop (binop5:binop) (exp1:exp) (exp2:exp) (annot5:annot)
- | Manyop (manyop5:manyop) (_:list exp) (annot5:annot)
- | Ite (exp1:exp) (exp2:exp) (exp3:exp) (annot5:annot).
-
 Inductive ty : Set := 
  | Ty_Bool : ty
  | Ty_BitVec (nat5:N)
  | Ty_Enum (enum_ty5:enum_id)
  | Ty_Array (ty1:ty) (ty2:ty).
+
+Inductive exp : Set := 
+ | Val (base_val5:base_val) (annot5:annot)
+ | Unop (unop5:unop) (exp5:exp) (annot5:annot)
+ | Binop (binop5:binop) (exp1:exp) (exp2:exp) (annot5:annot)
+ | Manyop (manyop5:manyop) (_:list exp) (annot5:annot)
+ | Ite (exp1:exp) (exp2:exp) (exp3:exp) (annot5:annot).
+
+Inductive valu : Set := 
+ | RegVal_Base (base_val5:base_val)
+ | RegVal_I (bvi5:Z) (int5:Z)
+ | RegVal_String (str5:string)
+ | RegVal_Unit : valu
+ | RegVal_NamedUnit (name5:register_name)
+ | RegVal_Vector (_:list valu)
+ | RegVal_List (_:list valu)
+ | RegVal_Struct (_:list (register_name * valu))
+ | RegVal_Poison : valu.
 
 Inductive accessor : Set := 
  | Field (name5:register_name).
@@ -116,9 +120,9 @@ Inductive smt : Set :=
  | Assert (exp5:exp)
  | DefineEnum (int5:Z).
 
-Definition accessor_list : Set := list accessor.
-
 Definition valu_option : Set := option valu.
+
+Definition accessor_list : Set := list accessor.
 
 Inductive event : Set := 
  | Smt (smt5:smt) (annot5:annot)
@@ -138,6 +142,8 @@ Inductive event : Set :=
  | SleepRequest (annot5:annot) (*r Arm sleep request *).
 
 Definition trc : Set := list event.
+
+Definition trcs : Set := list (list event).
 (** induction principles *)
 Section exp_rect.
 
@@ -146,7 +152,7 @@ Variables
   (P_exp : exp -> Prop).
 
 Hypothesis
-  (H_Val : forall (valu5:valu), forall (annot5:annot), P_exp (Val valu5 annot5))
+  (H_Val : forall (base_val5:base_val), forall (annot5:annot), P_exp (Val base_val5 annot5))
   (H_Unop : forall (unop5:unop), forall (exp5:exp), P_exp exp5 -> forall (annot5:annot), P_exp (Unop unop5 exp5 annot5))
   (H_Binop : forall (binop5:binop), forall (exp1:exp), P_exp exp1 -> forall (exp2:exp), P_exp exp2 -> forall (annot5:annot), P_exp (Binop binop5 exp1 exp2 annot5))
   (H_Manyop : forall (exp_list:list exp), P_list_exp exp_list -> forall (manyop5:manyop), forall (annot5:annot), P_exp (Manyop manyop5 exp_list annot5))
@@ -156,7 +162,7 @@ Hypothesis
 
 Fixpoint exp_ott_ind (n:exp) : P_exp n :=
   match n as x return P_exp x with
-  | (Val valu5 annot5) => H_Val valu5 annot5
+  | (Val base_val5 annot5) => H_Val base_val5 annot5
   | (Unop unop5 exp5 annot5) => H_Unop unop5 exp5 (exp_ott_ind exp5) annot5
   | (Binop binop5 exp1 exp2 annot5) => H_Binop binop5 exp1 (exp_ott_ind exp1) exp2 (exp_ott_ind exp2) annot5
   | (Manyop manyop5 exp_list annot5) => H_Manyop exp_list (((fix exp_list_ott_ind (exp_l:list exp) : P_list_exp exp_l := match exp_l as x return P_list_exp x with nil => H_list_exp_nil | cons exp1 xl => H_list_exp_cons exp1(exp_ott_ind exp1)xl (exp_list_ott_ind xl) end)) exp_list) manyop5 annot5
@@ -164,5 +170,69 @@ Fixpoint exp_ott_ind (n:exp) : P_exp n :=
 end.
 
 End exp_rect.
+
+(** substitutions *)
+Definition subst_val_base_val (base_val5:base_val) (vvar_6:var_name) (base_val_6:base_val) : base_val :=
+  match base_val_6 with
+  | (Val_Symbolic vvar5) => (if eq_var_name vvar5 vvar_6 then base_val5 else (Val_Symbolic vvar5))
+  | (Val_Bool bool5) => Val_Bool bool5
+  | (Val_Bits bv5) => Val_Bits bv5
+  | (Val_Enum enum5) => Val_Enum enum5
+end.
+
+Fixpoint subst_val_exp (base_val_6:base_val) (vvar5:var_name) (exp_6:exp) {struct exp_6} : exp :=
+  match exp_6 with
+  | (Val base_val5 annot5) => Val (subst_val_base_val base_val_6 vvar5 base_val5) annot5
+  | (Unop unop5 exp5 annot5) => Unop unop5 (subst_val_exp base_val_6 vvar5 exp5) annot5
+  | (Binop binop5 exp1 exp2 annot5) => Binop binop5 (subst_val_exp base_val_6 vvar5 exp1) (subst_val_exp base_val_6 vvar5 exp2) annot5
+  | (Manyop manyop5 exp_list annot5) => Manyop manyop5 (map (fun (exp_:exp) => (subst_val_exp base_val_6 vvar5 exp_)) exp_list) annot5
+  | (Ite exp1 exp2 exp3 annot5) => Ite (subst_val_exp base_val_6 vvar5 exp1) (subst_val_exp base_val_6 vvar5 exp2) (subst_val_exp base_val_6 vvar5 exp3) annot5
+end.
+
+Definition subst_val_smt (base_val5:base_val) (vvar_6:var_name) (smt5:smt) : smt :=
+  match smt5 with
+  | (DeclareConst vvar5 ty5) => DeclareConst vvar5 ty5
+  | (DefineConst vvar5 exp5) => DefineConst vvar5 (subst_val_exp base_val5 vvar_6 exp5)
+  | (Assert exp5) => Assert (subst_val_exp base_val5 vvar_6 exp5)
+  | (DefineEnum int5) => DefineEnum int5
+end.
+
+Fixpoint subst_val_valu (base_val_6:base_val) (vvar5:var_name) (addr5:valu) {struct addr5} : valu :=
+  match addr5 with
+  | (RegVal_Base base_val5) => RegVal_Base (subst_val_base_val base_val_6 vvar5 base_val5)
+  | (RegVal_I bvi5 int5) => RegVal_I bvi5 int5
+  | (RegVal_String str5) => RegVal_String str5
+  | RegVal_Unit => RegVal_Unit 
+  | (RegVal_NamedUnit name5) => RegVal_NamedUnit name5
+  | (RegVal_Vector valu_list) => RegVal_Vector (map (fun (valu_:valu) => (subst_val_valu base_val_6 vvar5 valu_)) valu_list)
+  | (RegVal_List valu_list) => RegVal_List (map (fun (valu_:valu) => (subst_val_valu base_val_6 vvar5 valu_)) valu_list)
+  | (RegVal_Struct selem_list) => RegVal_Struct selem_list
+  | RegVal_Poison => RegVal_Poison 
+end.
+
+Definition subst_val_event (base_val5:base_val) (vvar_6:var_name) (event5:event) : event :=
+  match event5 with
+  | (Smt smt5 annot5) => Smt (subst_val_smt base_val5 vvar_6 smt5) annot5
+  | (Branch int5 str5 annot5) => Branch int5 str5 annot5
+  | (ReadReg name5 accessor_list5 valu5 annot5) => ReadReg name5 accessor_list5 (subst_val_valu base_val5 vvar_6 valu5) annot5
+  | (WriteReg name5 accessor_list5 valu5 annot5) => WriteReg name5 accessor_list5 (subst_val_valu base_val5 vvar_6 valu5) annot5
+  | (ReadMem valu5 rkind addr num_bytes tag_value annot5) => ReadMem (subst_val_valu base_val5 vvar_6 valu5) (subst_val_valu base_val5 vvar_6 rkind) (subst_val_valu base_val5 vvar_6 addr) num_bytes tag_value annot5
+  | (WriteMem valu5 wkind addr data num_bytes tag_value annot5) => WriteMem (subst_val_valu base_val5 vvar_6 valu5) (subst_val_valu base_val5 vvar_6 wkind) (subst_val_valu base_val5 vvar_6 addr) (subst_val_valu base_val5 vvar_6 data) num_bytes tag_value annot5
+  | (BranchAddress addr annot5) => BranchAddress (subst_val_valu base_val5 vvar_6 addr) annot5
+  | (Barrier bkind annot5) => Barrier (subst_val_valu base_val5 vvar_6 bkind) annot5
+  | (CacheOp ckind addr annot5) => CacheOp (subst_val_valu base_val5 vvar_6 ckind) (subst_val_valu base_val5 vvar_6 addr) annot5
+  | (MarkReg name5 str5 annot5) => MarkReg name5 str5 annot5
+  | (Cycle annot5) => Cycle annot5
+  | (Instr opcode annot5) => Instr (subst_val_valu base_val5 vvar_6 opcode) annot5
+  | (Sleeping vvar5 annot5) => Sleeping vvar5 annot5
+  | (WakeRequest annot5) => WakeRequest annot5
+  | (SleepRequest annot5) => SleepRequest annot5
+end.
+
+
+Coercion RegVal_Base : base_val >-> valu.
+Definition base_val_to_exp (v : base_val) : exp := Val v Mk_annot.
+Coercion base_val_to_exp : base_val >-> exp.
+
 
 
